src/Bedrock/Field/Common/Arrays/MakeAccessSizes.v
@@ -22,9 +22,9 @@ Import AbstractInterpretation.Compilers.
 Import Types.Notations.
 
 Section __.
-  Context 
-    {width BW word mem locals env ext_spec varname_gen error}
-   `{parameters_sentinel : @parameters width BW word mem locals env ext_spec varname_gen error}.
+  Context
+    {width BW word mem locals ext_spec varname_gen error}
+   `{parameters_sentinel : @parameters width BW word mem locals ext_spec varname_gen error}.
   Existing Instances rep.Z rep.listZ_mem.
 
   Let all_access_sizes :=
