src/Bedrock/Field/Common/Arrays/MaxBounds.v
@@ -19,9 +19,9 @@ Local Open Scope Z_scope.
 Import ListNotations.
 
 Section MaxBounds.
-  Context 
-    {width BW word mem locals env ext_spec varname_gen error}
-   `{parameters_sentinel : @parameters width BW word mem locals env ext_spec varname_gen error}.
+  Context
+    {width BW word mem locals ext_spec varname_gen error}
+   `{parameters_sentinel : @parameters width BW word mem locals ext_spec varname_gen error}.
   Context {ok : ok}.
   Context (n : nat).
 
