src/Bedrock/Group/ScalarMult/LadderStep.v
@@ -33,11 +33,9 @@ End Gallina.
 Section __.
   Context {width: Z} {BW: Bitwidth width} {word: word.word width} {mem: map.map word Byte.byte}.
   Context {locals: map.map String.string word}.
-  Context {env: map.map String.string (list String.string * list String.string * Syntax.cmd)}.
   Context {ext_spec: bedrock2.Semantics.ExtSpec}.
   Context {word_ok : word.ok word} {mem_ok : map.ok mem}.
   Context {locals_ok : map.ok locals}.
-  Context {env_ok : map.ok env}.
   Context {ext_spec_ok : Semantics.ext_spec.ok ext_spec}.
   Context {field_parameters : FieldParameters}
           {field_representaton : FieldRepresentation}
@@ -115,7 +113,7 @@ Section __.
       <{ pred (nlet_eq
                  [X2_var; Z2_var; X3_var; Z3_var]
                  v k) }>.
-  Proof using env_ok ext_spec_ok locals_ok mem_ok word_ok.
+  Proof using ext_spec_ok locals_ok mem_ok word_ok.
     repeat straightline'.
     handle_call.
     apply H6.
